f[0] = 0, f[1] = 1, f[2] = 1, f[3] = 2

f[n] = f[n-1] + f[n-2] = f[n-2] + f[n-3] + f[n-2] = 2 * f[n-2] + f[n-3]

= 2 * (f[n-3] + f[n-4]) + f[n-3]) = 3*f[n-3] + 2 * f[n-4]

식을 보면  규칙이 보인다

## f[n] = f[k+1] * f[n-k] + f[k] * f[n-k-1]


이를 짝수일 때와 홀수일 때로 나누면 
### if n == 2k:
  f[2k] = f[k+1] * f[k] + f[k] * f[k-1]
  
  = f[k] ( f[k+1] + f[k-1] )
  
  = f[k] ( f[k] + f[k-1] + f[k-1])
  
  = f[k] ( 2 * f[k-1] + f[k] )

  ### f[2k] = f[k] ( 2 * f[k-1] + f[k] )

### if n == 2k + 1:
  f[2k+1] = f[k+1] * f[k+1] + f[k] * f[k] 
  
  = f[k+1]^2 + f[k]^2

  ### f[2k+1] = f[k+1]^2 + f[k]^2

이것을 재귀로 구현
리스트를 사용하면 메모리 초과지만 
